Some progress towards validated parsers
These parsers do not allow for failure and do not check bounds, instead
relying on validation of the input buffer.

examples/struct/keyvalue.pos/Test.fst
@@ -340,10 +340,6 @@ let validate =
 // the stack variables of a partially run parser being correct than to write proofs
 // about pure functions.
 
-// TODO: Another aspect to verify is that the bounds checks can be skipped. This
-// can be done even in pure F*, but is more obvious in effectful F* where we
-// prove safety of pointer arithmetic.
-
 // spec: fold over fully parsed store
 val fold_left_store: f:('a -> encoded_entry -> 'a) -> 'a -> s:store -> 'a
 let fold_left_store f acc s =
@@ -388,6 +384,38 @@ assume val parse_num_entries_valid : b:bytes{Some? (validate b)} ->
 assume val fold_left_buffer_ok: #t:Type -> f:(t -> encoded_entry -> t) -> acc:t -> b:bytes{Some? (validate b)} ->
     Lemma (fold_left_buffer f acc b ==
            fold_left_store f acc (parse_result (parse_abstract_store b)))
+
+
+(*! Skipping bounds checks due to validation *)
+
+// Another aspect to verify is that the bounds checks can be skipped. This
+// can be done even in pure F*, but is more obvious in effectful F* where we
+// prove safety of pointer arithmetic.
+
+// note that there are no bounds checks here; they are instead asserted and
+// proven through the validation
+let parse_valid_u16_array (b:bytes{Some? (validate_u16_array b)}) : a:u16_array{parse_result (parse_u16_array b) == a} =
+  // these asserts are for illustration only; in this simple example Z3 proves the
+  // right bounds automatically from the refinements on [slice].
+  assert (length b >= 2);
+  let len = u16_from_be (slice b 0 2) in
+  assert (length (slice b 2 (length b)) >= U16.v len);
+  let data = slice b 2 (2+U16.v len) in
+  U16Array len data
+
+let parse_valid_u32_array (b:bytes{Some? (validate_u32_array b)}) : a:u32_array{parse_result (parse_u32_array b) == a} =
+  let len = u32_from_be (slice b 0 4) in
+  let data = slice b 4 (4+U32.v len) in
+  U32Array len data
+
+assume val parse_valid_entry (b:bytes{Some? (validate_entry b)}) : e:encoded_entry{parse_result (parse_entry b) == e}
+  // TODO: unfortunately these validated parsers don't return how much data they
+  // consumed like normal parsers, so chaining them will require separately
+  // computing these lengths (based on the length of the array returned))
+
+  // TODO: the underlying reason is that a validated parser is a special case of
+  // a parser, but with a refinement on both the result type _and_ the input
+  // b:bytes, which can't even possibly be expressed using the [parser] type.
 
 (*! Parsing a cache *)
 
